qa/lean/Ragu/Instances/Boolean/ConditionalSelect.lean
@@ -37,9 +37,7 @@ def formal_instance : Core.Statements.GeneralFormalInstance where
       Circuits.Element.Mul.circuit,
       Circuits.Element.Mul.elaborated,
       Circuits.Element.Mul.main,
-      Circuits.Core.AllocMul.circuit,
-      Circuits.Core.AllocMul.elaborated,
-      Circuits.Core.AllocMul.main]
+      Circuits.Core.Mul.main]
     repeat (constructor; rfl)
     constructor
   same_output := by
@@ -55,8 +53,6 @@ def formal_instance : Core.Statements.GeneralFormalInstance where
       Circuits.Element.Mul.circuit,
       Circuits.Element.Mul.elaborated,
       Circuits.Element.Mul.main,
-      Circuits.Core.AllocMul.circuit,
-      Circuits.Core.AllocMul.elaborated,
-      Circuits.Core.AllocMul.main]
+      Circuits.Core.Mul.main]
 
 end Ragu.Instances.Boolean.ConditionalSelect
