qa/lean/Ragu/Instances/Point/AddIncomplete.lean
@@ -40,8 +40,8 @@ def formal_instance : Core.Statements.GeneralFormalInstance where
       Circuits.Element.Square.circuit, Circuits.Element.Square.elaborated, Circuits.Element.Square.main,
       Circuits.Element.DivNonzero.circuit, Circuits.Element.DivNonzero.elaborated,
       Circuits.Element.DivNonzero.main,
-      Circuits.Core.AllocMul.circuit, Circuits.Core.AllocMul.elaborated, Circuits.Core.AllocMul.main,
-      Circuits.Element.Mul.circuit, Circuits.Element.Mul.elaborated, Circuits.Element.Mul.main]
+      Circuits.Element.Mul.circuit, Circuits.Element.Mul.elaborated, Circuits.Element.Mul.main,
+      Circuits.Core.Mul.main]
     repeat (constructor; rfl)
     constructor
   same_output := by
@@ -53,8 +53,8 @@ def formal_instance : Core.Statements.GeneralFormalInstance where
       Circuits.Element.Square.circuit, Circuits.Element.Square.elaborated, Circuits.Element.Square.main,
       Circuits.Element.DivNonzero.circuit, Circuits.Element.DivNonzero.elaborated,
       Circuits.Element.DivNonzero.main,
-      Circuits.Core.AllocMul.circuit, Circuits.Core.AllocMul.elaborated, Circuits.Core.AllocMul.main,
-      Circuits.Element.Mul.circuit, Circuits.Element.Mul.elaborated, Circuits.Element.Mul.main]
+      Circuits.Element.Mul.circuit, Circuits.Element.Mul.elaborated, Circuits.Element.Mul.main,
+      Circuits.Core.Mul.main]
     repeat (constructor <;> congr)
 
 end Ragu.Instances.Point.AddIncomplete
