qa/lean/Ragu/Instances/Point/Double.lean
@@ -11,6 +11,7 @@ def deserializeInput (input : Vector (Expression (F p)) 2) : Var Circuits.Point.
 def serializeOutput (output : Var Circuits.Point.Spec.Point (F p)) : Vector (Expression (F p)) 2 :=
   #v[ output.x, output.y ]
 
+set_option maxHeartbeats 800000 in
 def formal_instance : Core.Statements.GeneralFormalInstance where
   p
   exportedOperations
@@ -34,8 +35,8 @@ def formal_instance : Core.Statements.GeneralFormalInstance where
       Circuits.Element.Square.circuit, Circuits.Element.Square.elaborated, Circuits.Element.Square.main,
       Circuits.Element.DivNonzero.circuit, Circuits.Element.DivNonzero.elaborated,
       Circuits.Element.DivNonzero.main,
-      Circuits.Core.AllocMul.circuit, Circuits.Core.AllocMul.elaborated, Circuits.Core.AllocMul.main,
-      Circuits.Element.Mul.circuit, Circuits.Element.Mul.elaborated, Circuits.Element.Mul.main]
+      Circuits.Element.Mul.circuit, Circuits.Element.Mul.elaborated, Circuits.Element.Mul.main,
+      Circuits.Core.Mul.main]
     repeat (constructor; rfl)
     constructor
   same_output := by
@@ -48,7 +49,6 @@ def formal_instance : Core.Statements.GeneralFormalInstance where
       Circuits.Element.Square.circuit, Circuits.Element.Square.elaborated, Circuits.Element.Square.main,
       Circuits.Element.DivNonzero.circuit, Circuits.Element.DivNonzero.elaborated,
       Circuits.Element.DivNonzero.main,
-      Circuits.Core.AllocMul.circuit, Circuits.Core.AllocMul.elaborated, Circuits.Core.AllocMul.main,
       Circuits.Element.Mul.circuit, Circuits.Element.Mul.elaborated, Circuits.Element.Mul.main]
     constructor <;> rfl
 end Ragu.Instances.Point.Double
