qa/lean/Ragu/Instances/Point/DoubleAndAddIncomplete.lean
@@ -46,9 +46,7 @@ def formal_instance : Core.Statements.GeneralFormalInstance where
       Circuits.Element.Mul.circuit,
       Circuits.Element.Mul.elaborated,
       Circuits.Element.Mul.main,
-      Circuits.Core.AllocMul.circuit,
-      Circuits.Core.AllocMul.elaborated,
-      Circuits.Core.AllocMul.main]
+      Circuits.Core.Mul.main]
     repeat (constructor; rfl)
     constructor
   same_output := by
@@ -70,9 +68,7 @@ def formal_instance : Core.Statements.GeneralFormalInstance where
       Circuits.Element.Mul.circuit,
       Circuits.Element.Mul.elaborated,
       Circuits.Element.Mul.main,
-      Circuits.Core.AllocMul.circuit,
-      Circuits.Core.AllocMul.elaborated,
-      Circuits.Core.AllocMul.main]
+      Circuits.Core.Mul.main]
     refine ⟨?_, rfl⟩
     rfl
 
